\documentclass{amsart}

\usepackage{graphicx}
\usepackage{verbatim}
\usepackage{amssymb}
\usepackage{tikz}
\usepackage{tikz-qtree}
\usepackage[margin=1in]{geometry}

\def\epsilon{\varepsilon}
\def\prob#1{P\left[#1\right]}
\def\expt#1{E\left[#1\right]}
\def\var#1{\mbox{Var}\left[#1\right]}
\def\cov#1{\mbox{Cov}\left(#1\right)}
\def\bin#1#2{\begin{pmatrix} #1 \\ #2 \end{pmatrix}}
\def\v#1{\mathbf{#1}}

\DeclareMathOperator*{\argmin}{arg\,min}

\title{Math\\600.475 Machine Learning}

\author{Anthony Burzillo\\aburzil1@jhu.edu}

\begin{document}

\maketitle

\def\touches#1#2{\mbox{touches}_{#1}{\left(#2\right)}}
\def\color#1{\mbox{color}{\left(#1\right)}}
\def\colorp#1{\mbox{color}^*{\left(#1\right)}}
\def\size#1{\mbox{size}{\left(#1\right)}}

Suppose we have a game $G$ for which we would like to determine $E(G)$. Let $k$ be the komi, $p_b$ and $p_w$ the prisoners
held by black and white, respectively, and the true final score $S$. Define $\touches{ e }{ b }$ to be the indicator function
taking the value 1 when the territory $e$ touches the block $b$. Define $\color{ b }$ to be the indicator function taking the
value 1 when the block $b$ is white. Similarly, define $\colorp{ b }$ to be the function taking the value -1 when $b$ is black and
1 when $b$ is white. Let $\size{ e }$ return the size of the territory or block $e$. The energy function runs algorithmically as follows:
\begin{enumerate}
  \item For each block $b_i$ calculate a feature vector $\v{ x }_i \in \mathbb{ R }^n$.
  \item Calculate $r_i = \v{ v } [W(\v{ x }_i + \v{ a }) + \v{ b }]$ for each $i$.
  \item For each territory $e_i$ compute
    \begin{align*}
      &N_b^{ (i) } = \sum_{ j = 1 }^n (1 - \color{ b_j }) \touches{ e_i }{ b_j }
      &N_w^{ (i) } = \sum_{ j = 1 }^n \color{ b_j } \touches{ e_i }{ b_j }\\
      &R_b^{ (i) } = \sum_{ j = 1 }^n (1 - \color{ b_j }) \touches{ e_i }{ b_j } r_j
      &R_w^{ (i) } = \sum_{ j = 1 }^n \color{ b_j } \touches{ e_i }{ b_j } r_j
    \end{align*}
  \item Construct the vector $\v{ r }_i = \{ N_b^{ (i) }, N_w^{ (i) }, R_b^{ (i) }, R_w^{ (i) }, \size{ e_i } \}$.
  \item Compute $s_i = \v{ g } [V(\v{ r }_i + \v{ c }) + \v{ d }]$.
  \item Compute $S^* = k - c_b + c_w + \sum_{ i = 1 }^t s_i$.
  \item We will assume that $r_i \neq 0$. Compute
    $$D = 2 \cdot \sum_{ i = 1 }^n \size{ b_i } \colorp{ b_i } r_i$$
  \item Output the energy $|S - (S^* + D)|$.
\end{enumerate}
We can write it out algebraically as
\begin{align*}
E(G) &= |E^*(G)| = |S - (S^* + D)|\\
  &= \left|S - \left(k - c_b + c_w + \sum_{ i = 1 }^t s_i
  + 2 \cdot \sum_{ i = 1 }^n \size{ b_i } \colorp{ b_i } r_i\right)\right|\\
  &= \left|S - k + c_b - c_w - \sum_{ i = 1 }^t \v{ g }[V(\v{ r }_i + \v{ c }) + \v{ d }]
  + 2 \cdot \sum_{ i = 1 }^n \size{ b_i } \colorp{ b_i } r_i\right|
\end{align*}
Therefore,
\begin{gather*}
\frac{ \partial E^*(G) }{ \partial \v{ g }_i }
  = -\sum_{ i = 1 }^t [V(\v{ r }_i + \v{ c }) + \v{ d }] \frac{ \partial }{ \partial \v{ g }_i } \v{ g }
\end{gather*}
\begin{gather*}
\frac{ \partial E^*(G) }{ \partial V_{ i j } }
  = -\sum_{ i = 1 }^t \v{ g } \left(\frac{ \partial }{ \partial V_{ i j } } V\right)(\v{ r }_i + \v{ c })
\end{gather*}
\begin{gather*}
\frac{ \partial E^*(G) }{ \partial \v{ c }_i }
  = - \sum_{ i = 1 }^t \v{ g } V \frac{ \partial }{ \partial \v{ c }_i } \v{ c }\\
\frac{ \partial E^*(G) }{ \partial \v{ d }_i } = \v{ g } \frac{ \partial }{ \partial \v{ d }_i } \v{ d }
\end{gather*}
Furthermore,
\begin{align*}
\frac{ \partial E^*(G) }{ \partial r_i }
  &= \sum_{ i = 1 }^t \v{ g } V \frac{ \partial }{ \partial r_i } \v{ r }_i
  + 2 \cdot \sum_{ i = 1 }^n \size{ b_i } \colorp{ b_i } \frac{ \partial }{ \partial r_i }  r_i\\
  &= \sum_{ i = 1 }^t \v{ g } V \left\{ 0, 0, \frac{ \partial }{ \partial r_i } R_b^{ (i) }, \frac{ \partial }{ \partial r_i } R_w^{ (i) }, 0 \right\}
  + 2 \cdot \sum_{ i = 1 }^n \size{ b_i } \colorp{ b_i } \frac{ \partial }{ \partial r_i }  r_i
\end{align*}
So then
\begin{gather*}
\frac{ \partial E^*(G) }{ \partial \v{ v }_i } = \sum_{ i = 1 }^t \v{ g } V
  \left\{ 0, 0, \sum_{ j = 1 }^n (1 - \color{ b_j }) \touches{ e_i }{ b_j } [W(\v{ x }_j + \v{ a }) + \v{ b }]
  \frac{ \partial }{ \partial \v{ v }_i } \v{ v },\right.\\
  \left.\sum_{ j = 1 }^n \color{ b_j } \touches{ e_i }{ b_j } [W(\v{ x }_j + \v{ a }) + \v{ b }]
  \frac{ \partial }{ \partial \v{ v }_i } \v{ v }, 0 \right\}\\
  + 2 \cdot \sum_{ i = 1 }^n \size{ b_i } \colorp{ b_i }  [W(\v{ x }_j + \v{ a }) + \v{ b }] \frac{ \partial }{ \partial \v{ v }_i } \v{ v }\\
\frac{ \partial E^*(G) }{ \partial W_{ i j } }  = \sum_{ i = 1 }^t \v{ g } V
  \left\{ 0, 0, \sum_{ j = 1 }^n (1 - \color{ b_j }) \touches{ e_i }{ b_j } \v{ v }
  \left(\frac{ \partial }{ \partial W_{ i j } } W\right) (\v{ x }_j + \v{ a }),\right.\\
  \left.\sum_{ j = 1 }^n \color{ b_j } \touches{ e_i }{ b_j } \v{ v }
  \left(\frac{ \partial }{ \partial W_{ i j } } W\right) (\v{ x }_j + \v{ a }), 0 \right\}\\
  + 2 \cdot \sum_{ i = 1 }^n \size{ b_i } \colorp{ b_i }  \v{ v }
  \left(\frac{ \partial }{ \partial W_{ i j } } W\right) (\v{ x }_j + \v{ a })\\
\frac{ \partial E^*(G) }{ \partial \v{ a }_i } = \sum_{ i = 1 }^t \v{ g } V
  \left\{ 0, 0, \sum_{ j = 1 }^n (1 - \color{ b_j }) \touches{ e_i }{ b_j }
  \v{ v } W \frac{ \partial }{ \partial \v{ a }_i } \v{ a },\right.\\
  \left.\sum_{ j = 1 }^n \color{ b_j } \touches{ e_i }{ b_j }
  \v{ v } W \frac{ \partial }{ \partial \v{ a }_i } \v{ a }, 0 \right\}\\
  + 2 \cdot \sum_{ i = 1 }^n \size{ b_i } \colorp{ b_i } \v{ v } W \frac{ \partial }{ \partial \v{ a }_i } \v{ a }\\
\frac{ \partial E^*(G) }{ \partial \v{ b }_i } = \sum_{ i = 1 }^t \v{ g } V
  \left\{ 0, 0, \sum_{ j = 1 }^n (1 - \color{ b_j }) \touches{ e_i }{ b_j }
  \v{ v } \frac{ \partial }{ \partial \v{ b }_i } \v{ b },\right.\\
  \left.\sum_{ j = 1 }^n \color{ b_j } \touches{ e_i }{ b_j }
  \v{ v } \frac{ \partial }{ \partial \v{ b }_i } \v{ b }, 0 \right\}\\
  + 2 \cdot \sum_{ i = 1 }^n \size{ b_i } \colorp{ b_i } \v{ v } \frac{ \partial }{ \partial \v{ b }_i } \v{ b }
\end{gather*}
Therefore, we can easily compute the same for $E(G)$ knowing that $d |x| / dx = x / |x|$.

\end{document}
